Split StateTransition into epoch/operations processing (see #51).

src/dafny/beacon/statetransition/StateTransition.s.dfy
@@ -22,6 +22,7 @@ include "../validators/Validators.dfy"
 include "../attestations/AttestationsTypes.dfy"
 include "../attestations/AttestationsHelpers.dfy"
 include "../Helpers.dfy"
+include "EpochProcessing.s.dfy"
 
 /**
  * State transition functional specification for the Beacon Chain.
@@ -38,6 +39,7 @@ module StateTransitionSpec {
     import opened AttestationsHelpers
     import opened BeaconHelpers
     import opened MathHelpers
+    import opened EpochProcessingSpec
 
     /**
      *  Collect pubkey in a list of validators.
@@ -54,37 +56,7 @@ module StateTransitionSpec {
             { xv[0].pubkey } + keysInValidators(xv[1..])
     }
 
-       /**
-     *  Collect pubkey in a list of validators.
-     *
-     *  @param  xv  A list of validators,
-     *  @returns    The sequence\list of keys helpd byt the validators in `xv`.
-     */
-    function method seqKeysInValidators(xv : seq<Validator>) : seq<BLSPubkey>
-        ensures |seqKeysInValidators(xv)| == |xv|
-        decreases xv
-    {
-        if |xv| == 0 then  
-            []
-        else 
-            [ xv[0].pubkey ] + seqKeysInValidators(xv[1..])
-    }
-
-    /**
-     *  Collect pubkey in a list of deposits.
-     *
-     *  @param  xd  A list of validators,
-     *  @returns    The sequence\list of keys held by the depositors in `xd`.
-     */
-    function method seqKeysInDeposits(xd : seq<Deposit>) : seq<BLSPubkey>
-        ensures |seqKeysInDeposits(xd)| == |xd|
-        decreases xd
-    {
-        if |xd| == 0 then  
-            []
-        else 
-            [ xd[0].data.pubkey ] + seqKeysInDeposits(xd[1..])
-    }
+   
 
     //  Specifications of finalisation of a state and forward to future slot.
 
@@ -239,105 +211,7 @@ module StateTransitionSpec {
                 resolveStateRoot(s)
     }
 
-    /**
-     *  Take into account deposits in a block.
-     *
-     *  @param  s           A beacon state.
-     *  @param  deposits    A list of deposits from a block body.
-     *  @returns            The state obtained after taking account the deposits in `body` from state `s` 
-     */
-    function updateDeposits(s: BeaconState, deposits: seq<Deposit>) : BeaconState 
-        requires s.eth1_deposit_index as int +  |deposits| < 0x10000000000000000 
-        requires |s.validators| == |s.balances|
-        requires |s.validators| + |deposits| <= VALIDATOR_REGISTRY_LIMIT as int
-        //requires forall i,j :: 0 <= i < j < |s.validators| ==> s.validators[i].pubkey != s.validators[j].pubkey
-
-        requires total_balances(s.balances) + total_deposits(deposits) < 0x10000000000000000 // less than total eth
-        //requires forall i :: 0 <= i < |s.validators| ==> s.balances[i] as int + get_deposit_total(s.validators[i].pubkey, deposits) as int < 0x10000000000000000
-        
-        //ensures updateDeposits(s, deposits).slot == s.slot 
-        //ensures updateDeposits(s, deposits).latest_block_header == s.latest_block_header
-        //ensures updateDeposits(s, deposits).block_roots == s.block_roots
-        //ensures updateDeposits(s, deposits).state_roots == s.state_roots
-
-        ensures updateDeposits(s, deposits).eth1_deposit_index == s.eth1_deposit_index  + |deposits| as uint64 
-        ensures |s.validators| <= |updateDeposits(s,deposits).validators| <= |s.validators| + |deposits| 
-        
-        // include properties ???
-        //ensures |updateDeposits(s,deposits).validators| == |updateDeposits(s,deposits).balances|        
-        //ensures |s.balances| <= |updateDeposits(s,deposits).balances| <= |s.balances| + |deposits| 
-
-        ensures total_balances(updateDeposits(s,deposits).balances) == total_balances(s.balances) + total_deposits(deposits)
-        
-         decreases |deposits|
-    {
-        if |deposits| == 0 then s
-        else 
-            //assert |deposits| > 0;
-            //assert forall i :: 0 <= i < |s.validators| ==> s.balances[i] as int + get_deposit_total(s.validators[i].pubkey, deposits) as int < 0x10000000000000000
-            //assert total_balances(s.balances) + total_deposits(deposits[..|deposits|-1]) < 0x10000000000000000 ;
-            //assert total_deposits(deposits[..|deposits|-1]) + total_deposits([deposits[|deposits|-1]]) == total_deposits(deposits) ;
-            //updateDeposits(s,deposits[..|deposits|-1])
-            //assert total_balances(s.balances) + total_deposits([deposits[|deposits|-1]]) < 0x10000000000000000;
-            //updateBalancesLemma(s,deposits);
-            //assert total_balances(s.balances) + total_deposits(deposits[..|deposits|-1]) < 0x10000000000000000;
-            //assert deposits[|deposits|-1].data.amount as int < total_deposits(deposits);
-            //assert total_balances(updateDeposits(s,deposits[..|deposits|-1]).balances) + deposits[|deposits|-1].data.amount as int < 0x10000000000000000;
-
-            updateBalTotalBySingleDeposit(updateDeposits(s,deposits[..|deposits|-1]), deposits[|deposits|-1]);
-
-            updateDeposit(updateDeposits(s,deposits[..|deposits|-1]),deposits[|deposits|-1])
-    }
-
-    /**
-     *  Take into account a single deposit from a block.
-     *
-     *  @param  s       A beacon state.
-     *  @param  d       A single deposit.
-     *  @returns        The state obtained after taking account the deposit `d` from state `s` 
-     */
-    function updateDeposit(s: BeaconState, d: Deposit) : BeaconState 
-        requires s.eth1_deposit_index as int +  1 < 0x10000000000000000 
-        requires |s.validators| == |s.balances|
-        requires |s.validators| + 1 <= VALIDATOR_REGISTRY_LIMIT as int
-        requires total_balances(s.balances) + d.data.amount as int < 0x10000000000000000
-        
-        //requires d.data.pubkey in seqKeysInValidators(s.validators) ==> s.balances[get_validator_index(seqKeysInValidators(s.validators), d.data.pubkey)] as int + d.data.amount as int < 0x10000000000000000
-        
-        ensures d.data.pubkey !in seqKeysInValidators(s.validators) ==> updateDeposit(s,d).validators == s.validators + [get_validator_from_deposit(d)]
-        ensures d.data.pubkey in seqKeysInValidators(s.validators)  ==> updateDeposit(s,d).validators == s.validators 
-        
-        ensures updateDeposit(s,d).eth1_deposit_index == s.eth1_deposit_index + 1
-        //ensures updateDeposit(s,d).slot == s.slot
-        //ensures updateDeposit(s,d).latest_block_header == s.latest_block_header
-        //ensures updateDeposit(s,d).block_roots == s.block_roots
-        //ensures updateDeposit(s,d).state_roots == s.state_roots
-
-        ensures |updateDeposit(s,d).validators| == |updateDeposit(s,d).balances|        // maybe include in property lemmas
-        ensures |s.validators| <= |updateDeposit(s,d).validators| <= |s.validators| + 1 // maybe include in property lemmas
-        ensures |s.balances| <= |updateDeposit(s,d).balances| <= |s.balances| + 1 // maybe include in property lemmas
-        ensures forall i :: 0 <= i < |s.balances| ==> s.balances[i] <= updateDeposit(s,d).balances[i]
-        //ensures total_balances(updateDeposit(s,d).balances) == total_balances(s.balances) + d.data.amount as int < 0x10000000000000000
-        // in lemma
-        
-    {
-        var pk := seqKeysInValidators(s.validators); 
-        
-        s.(
-            eth1_deposit_index := (s.eth1_deposit_index as int + 1) as uint64,
-            validators := if d.data.pubkey in pk then 
-                                s.validators // unchanged validator members
-                            else 
-                                validator_append(s.validators, get_validator_from_deposit(d)), //(s.validators + [get_validator_from_deposit(d)]),
-            balances := if d.data.pubkey in pk then 
-                                individualBalanceBoundMaintained(s.balances,d);
-                                //assert s.balances[get_validator_index(pk, d.data.pubkey)] as int + d.data.amount as int < 0x10000000000000000;
-                                increase_balance(s,get_validator_index(pk, d.data.pubkey),d.data.amount).balances
-                            else 
-                                balance_append(s.balances, d.data.amount) //s.balances + [d.data.amount]
-        )
-    }
-
+    
 
     /**
      *  Simplified first-cut specification of process_justification_and_finalization.
@@ -346,385 +220,298 @@ module StateTransitionSpec {
      *  @returns    The new state with justification checkpoints updated.
      *  
      */
-    function updateJustificationPrevEpoch(s: BeaconState) : BeaconState 
-        /** State's slot is not an Epoch boundary. */
-        requires s.slot % SLOTS_PER_EPOCH != 0
-        /** Justification bit are right-shifted and last two are not modified.
-            Bit0 (new checkpoint) and Bit1 (previous checkpoint) may be modified.
-         */
-        ensures get_current_epoch(s) > GENESIS_EPOCH + 1 ==> 
-            updateJustificationPrevEpoch(s).justification_bits[2..] == 
-                (s.justification_bits)[1..|s.justification_bits| - 1]
-    {
-        if  get_current_epoch(s) <= GENESIS_EPOCH + 1 then 
-            s 
-        else 
-            //  Right shift  justification_bits and prepend false
-            var newJustBits:= [false] + (s.justification_bits)[..JUSTIFICATION_BITS_LENGTH - 1];
-            //  Previous epoch checkpoint
-            //  Get attestations 
-            var matching_target_attestations := 
-                get_matching_target_attestations(s, get_previous_epoch(s));
-            var b1 := get_attesting_balance(s, matching_target_attestations) as nat * 3 
-                        >= get_total_active_balance(s) as nat * 2;
-            var c := CheckPoint(get_previous_epoch(s),
-                                        get_block_root(s, get_previous_epoch(s)));
-            s.(
-                current_justified_checkpoint := if b1 then c else s.current_justified_checkpoint,
-                previous_justified_checkpoint := s.current_justified_checkpoint,
-                justification_bits := if b1 then newJustBits[1 := true] else newJustBits
-            )
-    }
+    // function updateJustificationPrevEpoch(s: BeaconState) : BeaconState 
+    //     /** State's slot is not an Epoch boundary. */
+    //     requires s.slot % SLOTS_PER_EPOCH != 0
+    //     /** Justification bit are right-shifted and last two are not modified.
+    //         Bit0 (new checkpoint) and Bit1 (previous checkpoint) may be modified.
+    //      */
+    //     ensures get_current_epoch(s) > GENESIS_EPOCH + 1 ==> 
+    //         updateJustificationPrevEpoch(s).justification_bits[2..] == 
+    //             (s.justification_bits)[1..|s.justification_bits| - 1]
+    // {
+    //     if  get_current_epoch(s) <= GENESIS_EPOCH + 1 then 
+    //         s 
+    //     else 
+    //         //  Right shift  justification_bits and prepend false
+    //         var newJustBits:= [false] + (s.justification_bits)[..JUSTIFICATION_BITS_LENGTH - 1];
+    //         //  Previous epoch checkpoint
+    //         //  Get attestations 
+    //         var matching_target_attestations := 
+    //             get_matching_target_attestations(s, get_previous_epoch(s));
+    //         var b1 := get_attesting_balance(s, matching_target_attestations) as nat * 3 
+    //                     >= get_total_active_balance(s) as nat * 2;
+    //         var c := CheckPoint(get_previous_epoch(s),
+    //                                     get_block_root(s, get_previous_epoch(s)));
+    //         s.(
+    //             current_justified_checkpoint := if b1 then c else s.current_justified_checkpoint,
+    //             previous_justified_checkpoint := s.current_justified_checkpoint,
+    //             justification_bits := if b1 then newJustBits[1 := true] else newJustBits
+    //         )
+    // }
 
-    function updateJustification(s: BeaconState) : BeaconState
-        requires s.slot % SLOTS_PER_EPOCH != 0
-        // ensures updateJustification(s) == 
-        //     updateJustificationCurrentEpoch(updateJustificationPrevEpoch(s))
-        ensures get_current_epoch(s) > GENESIS_EPOCH + 1 ==> 
-            updateJustificationCurrentEpoch(s).justification_bits[1..] == 
-                (s.justification_bits)[1..|s.justification_bits|]
-    {
-        updateJustificationCurrentEpoch(updateJustificationPrevEpoch(s))
-    }
+    // function updateJustification(s: BeaconState) : BeaconState
+    //     requires s.slot % SLOTS_PER_EPOCH != 0
+    //     // ensures updateJustification(s) == 
+    //     //     updateJustificationCurrentEpoch(updateJustificationPrevEpoch(s))
+    //     ensures get_current_epoch(s) > GENESIS_EPOCH + 1 ==> 
+    //         updateJustificationCurrentEpoch(s).justification_bits[1..] == 
+    //             (s.justification_bits)[1..|s.justification_bits|]
+    // {
+    //     updateJustificationCurrentEpoch(updateJustificationPrevEpoch(s))
+    // }
 
-    function updateJustificationAndFinalisation(s: BeaconState) : BeaconState
-        requires s.slot % SLOTS_PER_EPOCH != 0
-    {
-        updateFinalisedCheckpoint(updateJustification(s))
-    }
+    // function updateJustificationAndFinalisation(s: BeaconState) : BeaconState
+    //     requires s.slot % SLOTS_PER_EPOCH != 0
+    // {
+    //     updateFinalisedCheckpoint(updateJustification(s))
+    // }
 
-    /**
-     *  Update related to the processing of current epoch.
-     */
-    function updateJustificationCurrentEpoch(s: BeaconState) : BeaconState 
-        /** State's slot is not an Epoch boundary. */
-        requires s.slot % SLOTS_PER_EPOCH != 0
-        /** Justification bit are right-shifted and last two are not modified.
-            Bit0 (new checkpoint) and Bit1 (previous checkpoint) may be modified.
-         */
-        ensures get_current_epoch(s) > GENESIS_EPOCH + 1 ==> 
-            updateJustificationCurrentEpoch(s).justification_bits[1..] == 
-                (s.justification_bits)[1..|s.justification_bits|]
-    {
-        if  get_current_epoch(s) <= GENESIS_EPOCH + 1 then 
-            s 
-        else 
-            //  Get attestations for current epoch
-            var matching_target_attestations := 
-                get_matching_target_attestations(s, get_current_epoch(s));
-            var b1 := get_attesting_balance(s, matching_target_attestations) as nat * 3 
-                        >= get_total_active_balance(s) as nat * 2;
-            var c := CheckPoint(get_current_epoch(s),
-                                        get_block_root(s, get_current_epoch(s)));
-            s.(
-                current_justified_checkpoint := if b1 then c else s.current_justified_checkpoint,
-                // previous_justified_checkpoint := s.current_justified_checkpoint,
-                justification_bits := if b1 then s.justification_bits[0 := true] else s.justification_bits
-            )
-    }
+    // /**
+    //  *  Update related to the processing of current epoch.
+    //  */
+    // function updateJustificationCurrentEpoch(s: BeaconState) : BeaconState 
+    //     /** State's slot is not an Epoch boundary. */
+    //     requires s.slot % SLOTS_PER_EPOCH != 0
+    //     /** Justification bit are right-shifted and last two are not modified.
+    //         Bit0 (new checkpoint) and Bit1 (previous checkpoint) may be modified.
+    //      */
+    //     ensures get_current_epoch(s) > GENESIS_EPOCH + 1 ==> 
+    //         updateJustificationCurrentEpoch(s).justification_bits[1..] == 
+    //             (s.justification_bits)[1..|s.justification_bits|]
+    // {
+    //     if  get_current_epoch(s) <= GENESIS_EPOCH + 1 then 
+    //         s 
+    //     else 
+    //         //  Get attestations for current epoch
+    //         var matching_target_attestations := 
+    //             get_matching_target_attestations(s, get_current_epoch(s));
+    //         var b1 := get_attesting_balance(s, matching_target_attestations) as nat * 3 
+    //                     >= get_total_active_balance(s) as nat * 2;
+    //         var c := CheckPoint(get_current_epoch(s),
+    //                                     get_block_root(s, get_current_epoch(s)));
+    //         s.(
+    //             current_justified_checkpoint := if b1 then c else s.current_justified_checkpoint,
+    //             // previous_justified_checkpoint := s.current_justified_checkpoint,
+    //             justification_bits := if b1 then s.justification_bits[0 := true] else s.justification_bits
+    //         )
+    // }
 
-    /**
-     *  Update a state finalised checkpoint.
-     *  @param  s   A state.
-     *  @returns    The new state after updating the status of finalised_checkpoint.
-     *  Epochs layout
-     *
-     *  | ............ | ........... | .......... | 
-     *  | ............ | ........... | .......... | 
-     *  e1             e2            e3           e4
-     *  bit[0]        bit[1]        bit[2]        bit[3]
-     *  current       previous
-     *
-    //  *  Python slice a[k:l] means: a[k] ... a[l -1]
-     */
-    function updateFinalisedCheckpoint(s: BeaconState) : BeaconState
-        ensures s.slot == updateFinalisedCheckpoint(s).slot
-    {
-        if get_current_epoch(s) <= GENESIS_EPOCH + 1 then 
-            s 
-        else 
-            var bits : seq<bool> := s.justification_bits;
-            var current_epoch := get_current_epoch(s);
-            if (all(bits[1..4]) && current_epoch >= 3 && s.previous_justified_checkpoint.epoch  == current_epoch - 3) then 
-                //  The 2nd/3rd/4th most recent epochs are justified, the 2nd using the 4th as source
-                s.(finalised_checkpoint := s.previous_justified_checkpoint) 
-            else if (all(bits[1..3]) && s.previous_justified_checkpoint.epoch == current_epoch - 2) then 
-                // The 2nd/3rd most recent epochs are justified, the 2nd using the 3rd as source
-                s.(finalised_checkpoint := s.previous_justified_checkpoint) 
-            else if (all(bits[0..3]) && s.current_justified_checkpoint.epoch == current_epoch - 2) then 
-                // The 1st/2nd/3rd most recent epochs are justified, the 1st using the 3rd as source
-                s.(finalised_checkpoint := s.current_justified_checkpoint) 
-            else if (false && all(bits[0..2]) && s.current_justified_checkpoint.epoch == current_epoch - 1) then 
-                // The 1st/2nd most recent epochs are justified, the 1st using the 2nd as source
-                s.(finalised_checkpoint := s.current_justified_checkpoint) 
-            else
-                s 
-    } 
+    // /**
+    //  *  Update a state finalised checkpoint.
+    //  *  @param  s   A state.
+    //  *  @returns    The new state after updating the status of finalised_checkpoint.
+    //  *  Epochs layout
+    //  *
+    //  *  | ............ | ........... | .......... | 
+    //  *  | ............ | ........... | .......... | 
+    //  *  e1             e2            e3           e4
+    //  *  bit[0]        bit[1]        bit[2]        bit[3]
+    //  *  current       previous
+    //  *
+    // //  *  Python slice a[k:l] means: a[k] ... a[l -1]
+    //  */
+    // function updateFinalisedCheckpoint(s: BeaconState) : BeaconState
+    //     ensures s.slot == updateFinalisedCheckpoint(s).slot
+    // {
+    //     if get_current_epoch(s) <= GENESIS_EPOCH + 1 then 
+    //         s 
+    //     else 
+    //         var bits : seq<bool> := s.justification_bits;
+    //         var current_epoch := get_current_epoch(s);
+    //         if (all(bits[1..4]) && current_epoch >= 3 && s.previous_justified_checkpoint.epoch  == current_epoch - 3) then 
+    //             //  The 2nd/3rd/4th most recent epochs are justified, the 2nd using the 4th as source
+    //             s.(finalised_checkpoint := s.previous_justified_checkpoint) 
+    //         else if (all(bits[1..3]) && s.previous_justified_checkpoint.epoch == current_epoch - 2) then 
+    //             // The 2nd/3rd most recent epochs are justified, the 2nd using the 3rd as source
+    //             s.(finalised_checkpoint := s.previous_justified_checkpoint) 
+    //         else if (all(bits[0..3]) && s.current_justified_checkpoint.epoch == current_epoch - 2) then 
+    //             // The 1st/2nd/3rd most recent epochs are justified, the 1st using the 3rd as source
+    //             s.(finalised_checkpoint := s.current_justified_checkpoint) 
+    //         else if (false && all(bits[0..2]) && s.current_justified_checkpoint.epoch == current_epoch - 1) then 
+    //             // The 1st/2nd most recent epochs are justified, the 1st using the 2nd as source
+    //             s.(finalised_checkpoint := s.current_justified_checkpoint) 
+    //         else
+    //             s 
+    // } 
 
-    /**
-     *  Final section of process_final_updates where attestations are rotated.
-     *  @param  s   A beacon state.
-     *  @returns    `s` with the attestations rotated.
-     */
-    function finalUpdates(s: BeaconState) : BeaconState
-    {
-        s.(
-            previous_epoch_attestations := s.current_epoch_attestations,
-            current_epoch_attestations := []
-        )
-    }
-    function total_deposits(deposits: seq<Deposit>): nat
-    {
-        if |deposits| == 0 then 0
-        //else deposits[0].data.amount as nat + total_deposits(deposits[1..])
-        else total_deposits(deposits[..|deposits|-1]) + deposits[|deposits|-1].data.amount as nat
-    }
-
-    function total_balances(bal: seq<Gwei>): nat
-    {
-        if |bal| == 0 then 0
-        else bal[0] as nat + total_balances(bal[1..])
-    }
-
-        /**
-     * Extract a validator from a single deposit.
-     *
-     *  @param  d       A single deposit.
-     *  @returns        A validator created from the deposit information
-     *
-     *  @note           The `effective_balance` is not an active field in the current model but the code
-     *                  to set this field is included as a comment for future reference.
-     */
-    function method get_validator_from_deposit(d: Deposit): Validator
-        ensures get_validator_from_deposit(d).effectiveBalance <= MAX_EFFECTIVE_BALANCE as Gwei
-    {
-        var amount := d.data.amount; 
-        var effective_balance := min((amount as int- amount as int % EFFECTIVE_BALANCE_INCREMENT) as nat, MAX_EFFECTIVE_BALANCE as nat);
-
-        Validator(d.data.pubkey, effective_balance as Gwei)
-    }
-
-    /**
-     *  Append a new validator
-     */
-    function method validator_append(sv: ListOfValidators, v: Validator): ListOfValidators
-        requires |sv| + 1 <= VALIDATOR_REGISTRY_LIMIT as int
-    {
-        sv + [v]
-    }
-    /**
-     *  Append a new balance entry
-     */
-    function method balance_append(sb: ListOfBalances, b: Gwei): ListOfBalances
-        requires |sb| + 1 <= VALIDATOR_REGISTRY_LIMIT as int
-    {
-        sb + [b]
-    }
-
-     /**
-     *  Get the index of a validator. 
-     *
-     *  @notes  Helper function as no alternative indexing functionality available.
-     *
-     */
-    function method get_validator_index(pk: seq<BLSPubkey>, pubkey: BLSPubkey) : ValidatorIndex
-        requires |pk| < VALIDATOR_REGISTRY_LIMIT as int
-        requires pubkey in pk
-        ensures get_validator_index(pk,pubkey) as int < |pk|
-        ensures pk[get_validator_index(pk,pubkey)] == pubkey
-        decreases pk
-    {
-        if pk[0] == pubkey then 0 as ValidatorIndex
-        else 1 + get_validator_index(pk[1..], pubkey)
-        // alternative reverse form
-        //if pk[|pk|-1] == pubkey then (|pk|-1) as ValidatorIndex
-        //else get_validator_index(pk[..|pk|-1], pubkey)
-
-    }
+    // /**
+    //  *  Final section of process_final_updates where attestations are rotated.
+    //  *  @param  s   A beacon state.
+    //  *  @returns    `s` with the attestations rotated.
+    //  */
+    // function finalUpdates(s: BeaconState) : BeaconState
+    // {
+    //     s.(
+    //         previous_epoch_attestations := s.current_epoch_attestations,
+    //         current_epoch_attestations := []
+    //     )
+    // }
 
 
-    // Beacon State Mutators
 
-    /** increase_balance
-     *  Increase the validator balance at index ``index`` by ``delta``.
-     *
-     *  @notes  The datatype Gwei has temporarily been changed from uint64 to nat so as to simplify the
-     *          properties required to process a deposit. Hence a further requires will be needed to prevent
-     *          overflow once this temporary simplification is removed.
-     *  
-     **/
-    function method increase_balance(s: BeaconState, index: ValidatorIndex, delta: Gwei): BeaconState 
-        requires index as int < |s.balances| 
-        requires s.balances[index] as int + delta as int < 0x10000000000000000
-        ensures |s.balances| == |increase_balance(s,index,delta).balances|
-        ensures increase_balance(s,index,delta).balances[index] == s.balances[index] + delta
-    {
-        s.(
-            balances := s.balances[index as int := (s.balances[index] + delta)]
-        )
-    }
     
     // Helper lemmas
 
 
-    lemma individualBalanceBoundMaintained(sb: seq<Gwei>, d: Deposit)
-        requires total_balances(sb) + d.data.amount as int < 0x10000000000000000
-        ensures forall i :: 0 <= i < |sb| ==> sb[i] as int + d.data.amount as int < 0x10000000000000000
-    {
-        if |sb| == 0 {
-            // Thanks Dafny
-        }
-        else {
-            //assert total_balances(sb) == sb[0] as int + total_balances(sb[1..]);
-            //assert sb[0] as int + d.data.amount as int < 0x10000000000000000;
-            //assert total_balances(sb[1..]) + d.data.amount as int < 0x10000000000000000;
-            individualBalanceBoundMaintained(sb[1..],d);
-        }
-    } 
+    // lemma individualBalanceBoundMaintained(sb: seq<Gwei>, d: Deposit)
+    //     requires total_balances(sb) + d.data.amount as int < 0x10000000000000000
+    //     ensures forall i :: 0 <= i < |sb| ==> sb[i] as int + d.data.amount as int < 0x10000000000000000
+    // {
+    //     if |sb| == 0 {
+    //         // Thanks Dafny
+    //     }
+    //     else {
+    //         //assert total_balances(sb) == sb[0] as int + total_balances(sb[1..]);
+    //         //assert sb[0] as int + d.data.amount as int < 0x10000000000000000;
+    //         //assert total_balances(sb[1..]) + d.data.amount as int < 0x10000000000000000;
+    //         individualBalanceBoundMaintained(sb[1..],d);
+    //     }
+    // } 
 
-    lemma updateBalTotalBySingleDeposit(s: BeaconState, d: Deposit)
-        requires s.eth1_deposit_index as int +  1 < 0x10000000000000000 
-        requires |s.validators| == |s.balances|
-        requires |s.validators| + 1 <= VALIDATOR_REGISTRY_LIMIT as int
-        requires total_balances(s.balances) + d.data.amount as int < 0x10000000000000000
+    // lemma updateBalTotalBySingleDeposit(s: BeaconState, d: Deposit)
+    //     requires s.eth1_deposit_index as int +  1 < 0x10000000000000000 
+    //     requires |s.validators| == |s.balances|
+    //     requires |s.validators| + 1 <= VALIDATOR_REGISTRY_LIMIT as int
+    //     requires total_balances(s.balances) + d.data.amount as int < 0x10000000000000000
         
-        ensures total_balances(updateDeposit(s,d).balances) == total_balances(s.balances) + d.data.amount as int < 0x10000000000000000
-        //ensures total_balances(updateDeposit(s,d).balances) == total_balances(s.balances) + total_deposits([d]) 
-    {
-        var pk := seqKeysInValidators(s.validators); 
-        if |s.balances| == 0 {
-            // Thanks Dafny
-        }
-        else {
-            if d.data.pubkey in pk {
-                var index := get_validator_index(pk, d.data.pubkey);
-                individualBalanceBoundMaintained(s.balances,d);
-                //assert updateDeposit(s,d).balances ==  increase_balance(s,index,d.data.amount).balances;
-                //assert increase_balance(s,index,d.data.amount).balances[index] == s.balances[index] + d.data.amount;
-                //assert forall i :: 0 <= i < |s.balances| && i != index as int ==> increase_balance(s,index,d.data.amount).balances[i] == s.balances[i];
-                //assert total_balances(updateDeposit(s,d).balances) == total_balances(increase_balance(s,index,d.data.amount).balances) ;
-                updateExistingBalance(s, index, d.data.amount);
-                //assert total_balances(updateDeposit(s,d).balances) == total_balances(s.balances) + d.data.amount as int ;
-            }
-            else {
-                //assert updateDeposit(s,d).balances == s.balances + [d.data.amount];
-                distBalancesProp(s.balances,[d.data.amount]);
-                //assert total_balances(s.balances + [d.data.amount]) == total_balances(s.balances) + total_balances([d.data.amount]);
-            }
-        }
-    }
+    //     ensures total_balances(updateDeposit(s,d).balances) == total_balances(s.balances) + d.data.amount as int < 0x10000000000000000
+    //     //ensures total_balances(updateDeposit(s,d).balances) == total_balances(s.balances) + total_deposits([d]) 
+    // {
+    //     var pk := seqKeysInValidators(s.validators); 
+    //     if |s.balances| == 0 {
+    //         // Thanks Dafny
+    //     }
+    //     else {
+    //         if d.data.pubkey in pk {
+    //             var index := get_validator_index(pk, d.data.pubkey);
+    //             individualBalanceBoundMaintained(s.balances,d);
+    //             //assert updateDeposit(s,d).balances ==  increase_balance(s,index,d.data.amount).balances;
+    //             //assert increase_balance(s,index,d.data.amount).balances[index] == s.balances[index] + d.data.amount;
+    //             //assert forall i :: 0 <= i < |s.balances| && i != index as int ==> increase_balance(s,index,d.data.amount).balances[i] == s.balances[i];
+    //             //assert total_balances(updateDeposit(s,d).balances) == total_balances(increase_balance(s,index,d.data.amount).balances) ;
+    //             updateExistingBalance(s, index, d.data.amount);
+    //             //assert total_balances(updateDeposit(s,d).balances) == total_balances(s.balances) + d.data.amount as int ;
+    //         }
+    //         else {
+    //             //assert updateDeposit(s,d).balances == s.balances + [d.data.amount];
+    //             distBalancesProp(s.balances,[d.data.amount]);
+    //             //assert total_balances(s.balances + [d.data.amount]) == total_balances(s.balances) + total_balances([d.data.amount]);
+    //         }
+    //     }
+    // }
 
-    lemma updateExistingBalance(s: BeaconState, index: ValidatorIndex, delta: Gwei)
-        requires index as int < |s.balances| 
-        requires s.balances[index] as int + delta as int < 0x10000000000000000
-        requires |s.balances| < VALIDATOR_REGISTRY_LIMIT as int
+    // lemma updateExistingBalance(s: BeaconState, index: ValidatorIndex, delta: Gwei)
+    //     requires index as int < |s.balances| 
+    //     requires s.balances[index] as int + delta as int < 0x10000000000000000
+    //     requires |s.balances| < VALIDATOR_REGISTRY_LIMIT as int
 
-        ensures total_balances(increase_balance(s,index,delta).balances) == total_balances(s.balances) + delta as int
-    {
-        //assert increase_balance(s,index,delta).balances[index] == s.balances[index] + delta;
-        //assert forall i :: 0 <= i < |s.balances| && i != index as int ==> increase_balance(s,index,delta).balances[i] == s.balances[i];
+    //     ensures total_balances(increase_balance(s,index,delta).balances) == total_balances(s.balances) + delta as int
+    // {
+    //     //assert increase_balance(s,index,delta).balances[index] == s.balances[index] + delta;
+    //     //assert forall i :: 0 <= i < |s.balances| && i != index as int ==> increase_balance(s,index,delta).balances[i] == s.balances[i];
 
-        if index as int < |s.balances|-1 {
-            assert increase_balance(s,index,delta).balances == increase_balance(s,index,delta).balances[..index] + [increase_balance(s,index,delta).balances[index]] + increase_balance(s,index,delta).balances[(index+1)..];
+    //     if index as int < |s.balances|-1 {
+    //         assert increase_balance(s,index,delta).balances == increase_balance(s,index,delta).balances[..index] + [increase_balance(s,index,delta).balances[index]] + increase_balance(s,index,delta).balances[(index+1)..];
                                                                 
-            //assert total_balances(increase_balance(s,index,delta).balances[..index]) == total_balances(s.balances[..index]);
-            //assert total_balances([increase_balance(s,index,delta).balances[index]]) == total_balances([s.balances[index]]) + delta as int;
-            //assert total_balances(increase_balance(s,index,delta).balances[(index+1)..]) == total_balances(s.balances[(index+1)..]);
+    //         //assert total_balances(increase_balance(s,index,delta).balances[..index]) == total_balances(s.balances[..index]);
+    //         //assert total_balances([increase_balance(s,index,delta).balances[index]]) == total_balances([s.balances[index]]) + delta as int;
+    //         //assert total_balances(increase_balance(s,index,delta).balances[(index+1)..]) == total_balances(s.balances[(index+1)..]);
 
-            //assert total_balances(increase_balance(s,index,delta).balances) == total_balances(increase_balance(s,index,delta).balances[..index] + [increase_balance(s,index,delta).balances[index]] + increase_balance(s,index,delta).balances[(index+1)..]);
+    //         //assert total_balances(increase_balance(s,index,delta).balances) == total_balances(increase_balance(s,index,delta).balances[..index] + [increase_balance(s,index,delta).balances[index]] + increase_balance(s,index,delta).balances[(index+1)..]);
 
-            distBalancesProp(increase_balance(s,index,delta).balances[..index], [increase_balance(s,index,delta).balances[index]]);
-            //assert total_balances(increase_balance(s,index,delta).balances[..index] + [increase_balance(s,index,delta).balances[index]]) == total_balances(increase_balance(s,index,delta).balances[..index]) + total_balances([increase_balance(s,index,delta).balances[index]]);
-            distBalancesProp(increase_balance(s,index,delta).balances[..index]+[increase_balance(s,index,delta).balances[index]], increase_balance(s,index,delta).balances[(index+1)..]);
-            //assert total_balances(increase_balance(s,index,delta).balances[..index] + [increase_balance(s,index,delta).balances[index]] + increase_balance(s,index,delta).balances[(index+1)..]) == total_balances(increase_balance(s,index,delta).balances[..index]) + total_balances([increase_balance(s,index,delta).balances[index]]) + total_balances(increase_balance(s,index,delta).balances[index+1..]);
+    //         distBalancesProp(increase_balance(s,index,delta).balances[..index], [increase_balance(s,index,delta).balances[index]]);
+    //         //assert total_balances(increase_balance(s,index,delta).balances[..index] + [increase_balance(s,index,delta).balances[index]]) == total_balances(increase_balance(s,index,delta).balances[..index]) + total_balances([increase_balance(s,index,delta).balances[index]]);
+    //         distBalancesProp(increase_balance(s,index,delta).balances[..index]+[increase_balance(s,index,delta).balances[index]], increase_balance(s,index,delta).balances[(index+1)..]);
+    //         //assert total_balances(increase_balance(s,index,delta).balances[..index] + [increase_balance(s,index,delta).balances[index]] + increase_balance(s,index,delta).balances[(index+1)..]) == total_balances(increase_balance(s,index,delta).balances[..index]) + total_balances([increase_balance(s,index,delta).balances[index]]) + total_balances(increase_balance(s,index,delta).balances[index+1..]);
 
-            //assert total_balances(increase_balance(s,index,delta).balances) == total_balances(increase_balance(s,index,delta).balances[..index]) + total_balances([increase_balance(s,index,delta).balances[index]]) + total_balances(increase_balance(s,index,delta).balances[index+1..]);
-            //assert total_balances(increase_balance(s,index,delta).balances) == total_balances(s.balances[..index]) + total_balances([s.balances[index]]) + delta as int + total_balances(s.balances[(index+1)..]);
+    //         //assert total_balances(increase_balance(s,index,delta).balances) == total_balances(increase_balance(s,index,delta).balances[..index]) + total_balances([increase_balance(s,index,delta).balances[index]]) + total_balances(increase_balance(s,index,delta).balances[index+1..]);
+    //         //assert total_balances(increase_balance(s,index,delta).balances) == total_balances(s.balances[..index]) + total_balances([s.balances[index]]) + delta as int + total_balances(s.balances[(index+1)..]);
 
-            //assert total_balances(increase_balance(s,index,delta).balances) == total_balances(s.balances[..index]) + total_balances([s.balances[index]]) + total_balances(s.balances[(index+1)..]) + delta as int;
+    //         //assert total_balances(increase_balance(s,index,delta).balances) == total_balances(s.balances[..index]) + total_balances([s.balances[index]]) + total_balances(s.balances[(index+1)..]) + delta as int;
 
-            assert s.balances == s.balances[..index] + [s.balances[index]] + s.balances[(index+1)..];
-            //assert total_balances(s.balances) == total_balances(s.balances[..index] + [s.balances[index]] + s.balances[(index+1)..]);
+    //         assert s.balances == s.balances[..index] + [s.balances[index]] + s.balances[(index+1)..];
+    //         //assert total_balances(s.balances) == total_balances(s.balances[..index] + [s.balances[index]] + s.balances[(index+1)..]);
 
-            distBalancesProp(s.balances[..index], [s.balances[index]]);
-            //assert total_balances(s.balances[..index] + [s.balances[index]]) == total_balances(s.balances[..index]) + total_balances([s.balances[index]]);
-            distBalancesProp(s.balances[..index]+[s.balances[index]], s.balances[(index+1)..]);
-            //assert total_balances(s.balances[..index] + [s.balances[index]] + s.balances[(index+1)..]) == total_balances(s.balances[..index]) + total_balances([s.balances[index]]) + total_balances(s.balances[index+1..]);
+    //         distBalancesProp(s.balances[..index], [s.balances[index]]);
+    //         //assert total_balances(s.balances[..index] + [s.balances[index]]) == total_balances(s.balances[..index]) + total_balances([s.balances[index]]);
+    //         distBalancesProp(s.balances[..index]+[s.balances[index]], s.balances[(index+1)..]);
+    //         //assert total_balances(s.balances[..index] + [s.balances[index]] + s.balances[(index+1)..]) == total_balances(s.balances[..index]) + total_balances([s.balances[index]]) + total_balances(s.balances[index+1..]);
 
-            //assert total_balances(increase_balance(s,index,delta).balances) == total_balances(s.balances) + delta as int;
-        }
-        else {
-            //assert index as int == |s.balances| - 1;
-            assert increase_balance(s,index,delta).balances == increase_balance(s,index,delta).balances[..index] + [increase_balance(s,index,delta).balances[index]];
+    //         //assert total_balances(increase_balance(s,index,delta).balances) == total_balances(s.balances) + delta as int;
+    //     }
+    //     else {
+    //         //assert index as int == |s.balances| - 1;
+    //         assert increase_balance(s,index,delta).balances == increase_balance(s,index,delta).balances[..index] + [increase_balance(s,index,delta).balances[index]];
                                                                 
-            //assert total_balances(increase_balance(s,index,delta).balances[..index]) == total_balances(s.balances[..index]);
-            //assert total_balances([increase_balance(s,index,delta).balances[index]]) == total_balances([s.balances[index]]) + delta as int;
+    //         //assert total_balances(increase_balance(s,index,delta).balances[..index]) == total_balances(s.balances[..index]);
+    //         //assert total_balances([increase_balance(s,index,delta).balances[index]]) == total_balances([s.balances[index]]) + delta as int;
             
-            //assert total_balances(increase_balance(s,index,delta).balances) == total_balances(increase_balance(s,index,delta).balances[..index] + [increase_balance(s,index,delta).balances[index]]);
+    //         //assert total_balances(increase_balance(s,index,delta).balances) == total_balances(increase_balance(s,index,delta).balances[..index] + [increase_balance(s,index,delta).balances[index]]);
 
-            distBalancesProp(increase_balance(s,index,delta).balances[..index], [increase_balance(s,index,delta).balances[index]]);
-            //assert total_balances(increase_balance(s,index,delta).balances[..index] + [increase_balance(s,index,delta).balances[index]]) == total_balances(increase_balance(s,index,delta).balances[..index]) + total_balances([increase_balance(s,index,delta).balances[index]]);
+    //         distBalancesProp(increase_balance(s,index,delta).balances[..index], [increase_balance(s,index,delta).balances[index]]);
+    //         //assert total_balances(increase_balance(s,index,delta).balances[..index] + [increase_balance(s,index,delta).balances[index]]) == total_balances(increase_balance(s,index,delta).balances[..index]) + total_balances([increase_balance(s,index,delta).balances[index]]);
             
             
-            //assert total_balances(increase_balance(s,index,delta).balances) == total_balances(s.balances[..index]) + total_balances([s.balances[index]]) + delta as int;
+    //         //assert total_balances(increase_balance(s,index,delta).balances) == total_balances(s.balances[..index]) + total_balances([s.balances[index]]) + delta as int;
 
-            assert s.balances == s.balances[..index] + [s.balances[index]] ;
-            //assert total_balances(s.balances) == total_balances(s.balances[..index] + [s.balances[index]]);
+    //         assert s.balances == s.balances[..index] + [s.balances[index]] ;
+    //         //assert total_balances(s.balances) == total_balances(s.balances[..index] + [s.balances[index]]);
 
-            distBalancesProp(s.balances[..index], [s.balances[index]]);
-            //assert total_balances(s.balances[..index] + [s.balances[index]]) == total_balances(s.balances[..index]) + total_balances([s.balances[index]]);
+    //         distBalancesProp(s.balances[..index], [s.balances[index]]);
+    //         //assert total_balances(s.balances[..index] + [s.balances[index]]) == total_balances(s.balances[..index]) + total_balances([s.balances[index]]);
             
-            //assert total_balances(increase_balance(s,index,delta).balances) == total_balances(s.balances) + delta as int;
-        }
-    }
+    //         //assert total_balances(increase_balance(s,index,delta).balances) == total_balances(s.balances) + delta as int;
+    //     }
+    // }
 
-    lemma distBalancesProp(sb1: seq<Gwei>, sb2: seq<Gwei>)
-        ensures total_balances(sb1 + sb2) == total_balances(sb1) + total_balances(sb2) 
-    {
-        if |sb1| == 0 {
-            assert sb1 + sb2 == sb2;
-        }
-        else {
-            var sb := sb1 + sb2;
-            //assert sb == [sb1[0]] +  sb1[1..] + sb2;
-            assert sb[1..] == sb1[1..] + sb2;
-            assert total_balances(sb) == sb[0] as int + total_balances(sb[1..]);
-            //assert total_balances(sb1 + sb2) == sb[0] as int + total_balances(sb1[1..] + sb2);
-            distBalancesProp(sb1[1..],sb2);
+    // lemma distBalancesProp(sb1: seq<Gwei>, sb2: seq<Gwei>)
+    //     ensures total_balances(sb1 + sb2) == total_balances(sb1) + total_balances(sb2) 
+    // {
+    //     if |sb1| == 0 {
+    //         assert sb1 + sb2 == sb2;
+    //     }
+    //     else {
+    //         var sb := sb1 + sb2;
+    //         //assert sb == [sb1[0]] +  sb1[1..] + sb2;
+    //         assert sb[1..] == sb1[1..] + sb2;
+    //         assert total_balances(sb) == sb[0] as int + total_balances(sb[1..]);
+    //         //assert total_balances(sb1 + sb2) == sb[0] as int + total_balances(sb1[1..] + sb2);
+    //         distBalancesProp(sb1[1..],sb2);
 
-        }
-    }
+    //     }
+    // }
 
-    lemma distDepositsProp(sd1: seq<Deposit>, sd2: seq<Deposit>)
-        ensures total_deposits(sd1 + sd2) == total_deposits(sd1) + total_deposits(sd2) 
-    {
-        if |sd2| == 0 {
-            assert sd1 + sd2 == sd1;
-        }
-        else {
-            var sd := sd1 + sd2;
-            //assert sd == sd1 + sd2[..|sd2|-1] +  [sd2[|sd2|-1]];
-            assert sd[..|sd|-1] == sd1 + sd2[..|sd2|-1] ;
-            assert total_deposits(sd) == total_deposits(sd[..|sd|-1]) + sd2[|sd2|-1].data.amount as int;
-            //assert total_deposits(sd1 + sd2) == total_deposits(sd1 + sd2[..|sd2|-1] ) + sd2[|sd2|-1].data.amount as int;
-            distDepositsProp(sd1, sd2[..|sd2|-1] );
-        }
-    }
-    lemma subsetDepositSumProp(deposits: seq<Deposit>, i: nat)
-        requires i <= |deposits|
-        ensures total_deposits(deposits[..i]) <= total_deposits(deposits);
-    {
-        if i == |deposits| {
-            assert deposits[..i] == deposits;
-        }
-        else {
-            //assert i < |deposits|;
-            assert deposits == deposits[..i] + deposits[i..];
-            assert total_deposits(deposits) == total_deposits(deposits[..i] + deposits[i..]);
-            distDepositsProp(deposits[..i], deposits[i..]);
-            //assert total_deposits(deposits[..i] + deposits[i..]) == total_deposits(deposits[..i]) + total_deposits(deposits[i..]); 
-        }
-    }
+    // lemma distDepositsProp(sd1: seq<Deposit>, sd2: seq<Deposit>)
+    //     ensures total_deposits(sd1 + sd2) == total_deposits(sd1) + total_deposits(sd2) 
+    // {
+    //     if |sd2| == 0 {
+    //         assert sd1 + sd2 == sd1;
+    //     }
+    //     else {
+    //         var sd := sd1 + sd2;
+    //         //assert sd == sd1 + sd2[..|sd2|-1] +  [sd2[|sd2|-1]];
+    //         assert sd[..|sd|-1] == sd1 + sd2[..|sd2|-1] ;
+    //         assert total_deposits(sd) == total_deposits(sd[..|sd|-1]) + sd2[|sd2|-1].data.amount as int;
+    //         //assert total_deposits(sd1 + sd2) == total_deposits(sd1 + sd2[..|sd2|-1] ) + sd2[|sd2|-1].data.amount as int;
+    //         distDepositsProp(sd1, sd2[..|sd2|-1] );
+    //     }
+    // }
+    // lemma subsetDepositSumProp(deposits: seq<Deposit>, i: nat)
+    //     requires i <= |deposits|
+    //     ensures total_deposits(deposits[..i]) <= total_deposits(deposits);
+    // {
+    //     if i == |deposits| {
+    //         assert deposits[..i] == deposits;
+    //     }
+    //     else {
+    //         //assert i < |deposits|;
+    //         assert deposits == deposits[..i] + deposits[i..];
+    //         assert total_deposits(deposits) == total_deposits(deposits[..i] + deposits[i..]);
+    //         distDepositsProp(deposits[..i], deposits[i..]);
+    //         //assert total_deposits(deposits[..i] + deposits[i..]) == total_deposits(deposits[..i]) + total_deposits(deposits[i..]); 
+    //     }
+    // }
 
     
 
