src/dafny/beacon/statetransition/EpochProcessing.s.dfy
@@ -1,0 +1,347 @@
+/*
+ * Copyright 2020 ConsenSys Software Inc.
+ *
+ * Licensed under the Apache License, Version 2.0 (the "License"); you may 
+ * not use this file except in compliance with the License. You may obtain 
+ * a copy of the License at http://www.apache.org/licenses/LICENSE-2.0
+ *
+ * Unless required by applicable law or agreed to in writing, software dis-
+ * tributed under the License is distributed on an "AS IS" BASIS, WITHOUT 
+ * WARRANTIES OR CONDITIONS OF ANY KIND, either express or implied. See the 
+ * License for the specific language governing permissions and limitations 
+ * under the License.
+ */
+
+include "../../utils/NativeTypes.dfy"
+include "../../utils/Eth2Types.dfy"
+include "../../utils/Helpers.dfy"
+include "../../utils/MathHelpers.dfy"
+include "../../ssz/Constants.dfy"
+include "../BeaconChainTypes.dfy"
+include "../validators/Validators.dfy"
+include "../attestations/AttestationsTypes.dfy"
+include "../attestations/AttestationsHelpers.dfy"
+include "../Helpers.dfy"
+
+/**
+ * State transition functional specification for the Beacon Chain.
+ */
+module EpochProcessingSpec {
+    
+    //  Import some constants, types and beacon chain helpers.
+    import opened NativeTypes
+    import opened Eth2Types
+    import opened Constants
+    import opened BeaconChainTypes
+    import opened Validators
+    import opened AttestationsTypes
+    import opened AttestationsHelpers
+    import opened BeaconHelpers
+    import opened MathHelpers
+
+    //  Specifications of finalisation of a state and forward to future slot.
+
+   
+    /**
+     *  Simplified first-cut specification of process_justification_and_finalization.
+     *
+     *  @param  s   A beacon state the slot of which is not an Epoch boundary. 
+     *  @returns    The new state with justification checkpoints updated.
+     *  
+     */
+    function updateJustificationPrevEpoch(s: BeaconState) : BeaconState 
+        /** State's slot is not an Epoch boundary. */
+        requires s.slot % SLOTS_PER_EPOCH != 0
+        /** Justification bit are right-shifted and last two are not modified.
+            Bit0 (new checkpoint) and Bit1 (previous checkpoint) may be modified.
+         */
+        ensures get_current_epoch(s) > GENESIS_EPOCH + 1 ==> 
+            updateJustificationPrevEpoch(s).justification_bits[2..] == 
+                (s.justification_bits)[1..|s.justification_bits| - 1]
+    {
+        if  get_current_epoch(s) <= GENESIS_EPOCH + 1 then 
+            s 
+        else 
+            //  Right shift  justification_bits and prepend false
+            var newJustBits:= [false] + (s.justification_bits)[..JUSTIFICATION_BITS_LENGTH - 1];
+            //  Previous epoch checkpoint
+            //  Get attestations 
+            var matching_target_attestations := 
+                get_matching_target_attestations(s, get_previous_epoch(s));
+            var b1 := get_attesting_balance(s, matching_target_attestations) as nat * 3 
+                        >= get_total_active_balance(s) as nat * 2;
+            var c := CheckPoint(get_previous_epoch(s),
+                                        get_block_root(s, get_previous_epoch(s)));
+            s.(
+                current_justified_checkpoint := if b1 then c else s.current_justified_checkpoint,
+                previous_justified_checkpoint := s.current_justified_checkpoint,
+                justification_bits := if b1 then newJustBits[1 := true] else newJustBits
+            )
+    }
+
+    function updateJustification(s: BeaconState) : BeaconState
+        requires s.slot % SLOTS_PER_EPOCH != 0
+        // ensures updateJustification(s) == 
+        //     updateJustificationCurrentEpoch(updateJustificationPrevEpoch(s))
+        ensures get_current_epoch(s) > GENESIS_EPOCH + 1 ==> 
+            updateJustificationCurrentEpoch(s).justification_bits[1..] == 
+                (s.justification_bits)[1..|s.justification_bits|]
+    {
+        updateJustificationCurrentEpoch(updateJustificationPrevEpoch(s))
+    }
+
+    function updateJustificationAndFinalisation(s: BeaconState) : BeaconState
+        requires s.slot % SLOTS_PER_EPOCH != 0
+    {
+        updateFinalisedCheckpoint(updateJustification(s))
+    }
+
+    /**
+     *  Update related to the processing of current epoch.
+     */
+    function updateJustificationCurrentEpoch(s: BeaconState) : BeaconState 
+        /** State's slot is not an Epoch boundary. */
+        requires s.slot % SLOTS_PER_EPOCH != 0
+        /** Justification bit are right-shifted and last two are not modified.
+            Bit0 (new checkpoint) and Bit1 (previous checkpoint) may be modified.
+         */
+        ensures get_current_epoch(s) > GENESIS_EPOCH + 1 ==> 
+            updateJustificationCurrentEpoch(s).justification_bits[1..] == 
+                (s.justification_bits)[1..|s.justification_bits|]
+    {
+        if  get_current_epoch(s) <= GENESIS_EPOCH + 1 then 
+            s 
+        else 
+            //  Get attestations for current epoch
+            var matching_target_attestations := 
+                get_matching_target_attestations(s, get_current_epoch(s));
+            var b1 := get_attesting_balance(s, matching_target_attestations) as nat * 3 
+                        >= get_total_active_balance(s) as nat * 2;
+            var c := CheckPoint(get_current_epoch(s),
+                                        get_block_root(s, get_current_epoch(s)));
+            s.(
+                current_justified_checkpoint := if b1 then c else s.current_justified_checkpoint,
+                // previous_justified_checkpoint := s.current_justified_checkpoint,
+                justification_bits := if b1 then s.justification_bits[0 := true] else s.justification_bits
+            )
+    }
+
+    /**
+     *  Update a state finalised checkpoint.
+     *  @param  s   A state.
+     *  @returns    The new state after updating the status of finalised_checkpoint.
+     *  Epochs layout
+     *
+     *  | ............ | ........... | .......... | 
+     *  | ............ | ........... | .......... | 
+     *  e1             e2            e3           e4
+     *  bit[0]        bit[1]        bit[2]        bit[3]
+     *  current       previous
+     *
+    //  *  Python slice a[k:l] means: a[k] ... a[l -1]
+     */
+    function updateFinalisedCheckpoint(s: BeaconState) : BeaconState
+        ensures s.slot == updateFinalisedCheckpoint(s).slot
+    {
+        if get_current_epoch(s) <= GENESIS_EPOCH + 1 then 
+            s 
+        else 
+            var bits : seq<bool> := s.justification_bits;
+            var current_epoch := get_current_epoch(s);
+            if (all(bits[1..4]) && current_epoch >= 3 && s.previous_justified_checkpoint.epoch  == current_epoch - 3) then 
+                //  The 2nd/3rd/4th most recent epochs are justified, the 2nd using the 4th as source
+                s.(finalised_checkpoint := s.previous_justified_checkpoint) 
+            else if (all(bits[1..3]) && s.previous_justified_checkpoint.epoch == current_epoch - 2) then 
+                // The 2nd/3rd most recent epochs are justified, the 2nd using the 3rd as source
+                s.(finalised_checkpoint := s.previous_justified_checkpoint) 
+            else if (all(bits[0..3]) && s.current_justified_checkpoint.epoch == current_epoch - 2) then 
+                // The 1st/2nd/3rd most recent epochs are justified, the 1st using the 3rd as source
+                s.(finalised_checkpoint := s.current_justified_checkpoint) 
+            else if (false && all(bits[0..2]) && s.current_justified_checkpoint.epoch == current_epoch - 1) then 
+                // The 1st/2nd most recent epochs are justified, the 1st using the 2nd as source
+                s.(finalised_checkpoint := s.current_justified_checkpoint) 
+            else
+                s 
+    } 
+
+    /**
+     *  Final section of process_final_updates where attestations are rotated.
+     *  @param  s   A beacon state.
+     *  @returns    `s` with the attestations rotated.
+     */
+    function finalUpdates(s: BeaconState) : BeaconState
+    {
+        s.(
+            previous_epoch_attestations := s.current_epoch_attestations,
+            current_epoch_attestations := []
+        )
+    }
+
+
+
+    
+    // // Helper lemmas
+
+
+    // lemma individualBalanceBoundMaintained(sb: seq<Gwei>, d: Deposit)
+    //     requires total_balances(sb) + d.data.amount as int < 0x10000000000000000
+    //     ensures forall i :: 0 <= i < |sb| ==> sb[i] as int + d.data.amount as int < 0x10000000000000000
+    // {
+    //     if |sb| == 0 {
+    //         // Thanks Dafny
+    //     }
+    //     else {
+    //         //assert total_balances(sb) == sb[0] as int + total_balances(sb[1..]);
+    //         //assert sb[0] as int + d.data.amount as int < 0x10000000000000000;
+    //         //assert total_balances(sb[1..]) + d.data.amount as int < 0x10000000000000000;
+    //         individualBalanceBoundMaintained(sb[1..],d);
+    //     }
+    // } 
+
+    // lemma updateBalTotalBySingleDeposit(s: BeaconState, d: Deposit)
+    //     requires s.eth1_deposit_index as int +  1 < 0x10000000000000000 
+    //     requires |s.validators| == |s.balances|
+    //     requires |s.validators| + 1 <= VALIDATOR_REGISTRY_LIMIT as int
+    //     requires total_balances(s.balances) + d.data.amount as int < 0x10000000000000000
+        
+    //     ensures total_balances(updateDeposit(s,d).balances) == total_balances(s.balances) + d.data.amount as int < 0x10000000000000000
+    //     //ensures total_balances(updateDeposit(s,d).balances) == total_balances(s.balances) + total_deposits([d]) 
+    // {
+    //     var pk := seqKeysInValidators(s.validators); 
+    //     if |s.balances| == 0 {
+    //         // Thanks Dafny
+    //     }
+    //     else {
+    //         if d.data.pubkey in pk {
+    //             var index := get_validator_index(pk, d.data.pubkey);
+    //             individualBalanceBoundMaintained(s.balances,d);
+    //             //assert updateDeposit(s,d).balances ==  increase_balance(s,index,d.data.amount).balances;
+    //             //assert increase_balance(s,index,d.data.amount).balances[index] == s.balances[index] + d.data.amount;
+    //             //assert forall i :: 0 <= i < |s.balances| && i != index as int ==> increase_balance(s,index,d.data.amount).balances[i] == s.balances[i];
+    //             //assert total_balances(updateDeposit(s,d).balances) == total_balances(increase_balance(s,index,d.data.amount).balances) ;
+    //             updateExistingBalance(s, index, d.data.amount);
+    //             //assert total_balances(updateDeposit(s,d).balances) == total_balances(s.balances) + d.data.amount as int ;
+    //         }
+    //         else {
+    //             //assert updateDeposit(s,d).balances == s.balances + [d.data.amount];
+    //             distBalancesProp(s.balances,[d.data.amount]);
+    //             //assert total_balances(s.balances + [d.data.amount]) == total_balances(s.balances) + total_balances([d.data.amount]);
+    //         }
+    //     }
+    // }
+
+    // lemma updateExistingBalance(s: BeaconState, index: ValidatorIndex, delta: Gwei)
+    //     requires index as int < |s.balances| 
+    //     requires s.balances[index] as int + delta as int < 0x10000000000000000
+    //     requires |s.balances| < VALIDATOR_REGISTRY_LIMIT as int
+
+    //     ensures total_balances(increase_balance(s,index,delta).balances) == total_balances(s.balances) + delta as int
+    // {
+    //     //assert increase_balance(s,index,delta).balances[index] == s.balances[index] + delta;
+    //     //assert forall i :: 0 <= i < |s.balances| && i != index as int ==> increase_balance(s,index,delta).balances[i] == s.balances[i];
+
+    //     if index as int < |s.balances|-1 {
+    //         assert increase_balance(s,index,delta).balances == increase_balance(s,index,delta).balances[..index] + [increase_balance(s,index,delta).balances[index]] + increase_balance(s,index,delta).balances[(index+1)..];
+                                                                
+    //         //assert total_balances(increase_balance(s,index,delta).balances[..index]) == total_balances(s.balances[..index]);
+    //         //assert total_balances([increase_balance(s,index,delta).balances[index]]) == total_balances([s.balances[index]]) + delta as int;
+    //         //assert total_balances(increase_balance(s,index,delta).balances[(index+1)..]) == total_balances(s.balances[(index+1)..]);
+
+    //         //assert total_balances(increase_balance(s,index,delta).balances) == total_balances(increase_balance(s,index,delta).balances[..index] + [increase_balance(s,index,delta).balances[index]] + increase_balance(s,index,delta).balances[(index+1)..]);
+
+    //         distBalancesProp(increase_balance(s,index,delta).balances[..index], [increase_balance(s,index,delta).balances[index]]);
+    //         //assert total_balances(increase_balance(s,index,delta).balances[..index] + [increase_balance(s,index,delta).balances[index]]) == total_balances(increase_balance(s,index,delta).balances[..index]) + total_balances([increase_balance(s,index,delta).balances[index]]);
+    //         distBalancesProp(increase_balance(s,index,delta).balances[..index]+[increase_balance(s,index,delta).balances[index]], increase_balance(s,index,delta).balances[(index+1)..]);
+    //         //assert total_balances(increase_balance(s,index,delta).balances[..index] + [increase_balance(s,index,delta).balances[index]] + increase_balance(s,index,delta).balances[(index+1)..]) == total_balances(increase_balance(s,index,delta).balances[..index]) + total_balances([increase_balance(s,index,delta).balances[index]]) + total_balances(increase_balance(s,index,delta).balances[index+1..]);
+
+    //         //assert total_balances(increase_balance(s,index,delta).balances) == total_balances(increase_balance(s,index,delta).balances[..index]) + total_balances([increase_balance(s,index,delta).balances[index]]) + total_balances(increase_balance(s,index,delta).balances[index+1..]);
+    //         //assert total_balances(increase_balance(s,index,delta).balances) == total_balances(s.balances[..index]) + total_balances([s.balances[index]]) + delta as int + total_balances(s.balances[(index+1)..]);
+
+    //         //assert total_balances(increase_balance(s,index,delta).balances) == total_balances(s.balances[..index]) + total_balances([s.balances[index]]) + total_balances(s.balances[(index+1)..]) + delta as int;
+
+    //         assert s.balances == s.balances[..index] + [s.balances[index]] + s.balances[(index+1)..];
+    //         //assert total_balances(s.balances) == total_balances(s.balances[..index] + [s.balances[index]] + s.balances[(index+1)..]);
+
+    //         distBalancesProp(s.balances[..index], [s.balances[index]]);
+    //         //assert total_balances(s.balances[..index] + [s.balances[index]]) == total_balances(s.balances[..index]) + total_balances([s.balances[index]]);
+    //         distBalancesProp(s.balances[..index]+[s.balances[index]], s.balances[(index+1)..]);
+    //         //assert total_balances(s.balances[..index] + [s.balances[index]] + s.balances[(index+1)..]) == total_balances(s.balances[..index]) + total_balances([s.balances[index]]) + total_balances(s.balances[index+1..]);
+
+    //         //assert total_balances(increase_balance(s,index,delta).balances) == total_balances(s.balances) + delta as int;
+    //     }
+    //     else {
+    //         //assert index as int == |s.balances| - 1;
+    //         assert increase_balance(s,index,delta).balances == increase_balance(s,index,delta).balances[..index] + [increase_balance(s,index,delta).balances[index]];
+                                                                
+    //         //assert total_balances(increase_balance(s,index,delta).balances[..index]) == total_balances(s.balances[..index]);
+    //         //assert total_balances([increase_balance(s,index,delta).balances[index]]) == total_balances([s.balances[index]]) + delta as int;
+            
+    //         //assert total_balances(increase_balance(s,index,delta).balances) == total_balances(increase_balance(s,index,delta).balances[..index] + [increase_balance(s,index,delta).balances[index]]);
+
+    //         distBalancesProp(increase_balance(s,index,delta).balances[..index], [increase_balance(s,index,delta).balances[index]]);
+    //         //assert total_balances(increase_balance(s,index,delta).balances[..index] + [increase_balance(s,index,delta).balances[index]]) == total_balances(increase_balance(s,index,delta).balances[..index]) + total_balances([increase_balance(s,index,delta).balances[index]]);
+            
+            
+    //         //assert total_balances(increase_balance(s,index,delta).balances) == total_balances(s.balances[..index]) + total_balances([s.balances[index]]) + delta as int;
+
+    //         assert s.balances == s.balances[..index] + [s.balances[index]] ;
+    //         //assert total_balances(s.balances) == total_balances(s.balances[..index] + [s.balances[index]]);
+
+    //         distBalancesProp(s.balances[..index], [s.balances[index]]);
+    //         //assert total_balances(s.balances[..index] + [s.balances[index]]) == total_balances(s.balances[..index]) + total_balances([s.balances[index]]);
+            
+    //         //assert total_balances(increase_balance(s,index,delta).balances) == total_balances(s.balances) + delta as int;
+    //     }
+    // }
+
+    // lemma distBalancesProp(sb1: seq<Gwei>, sb2: seq<Gwei>)
+    //     ensures total_balances(sb1 + sb2) == total_balances(sb1) + total_balances(sb2) 
+    // {
+    //     if |sb1| == 0 {
+    //         assert sb1 + sb2 == sb2;
+    //     }
+    //     else {
+    //         var sb := sb1 + sb2;
+    //         //assert sb == [sb1[0]] +  sb1[1..] + sb2;
+    //         assert sb[1..] == sb1[1..] + sb2;
+    //         assert total_balances(sb) == sb[0] as int + total_balances(sb[1..]);
+    //         //assert total_balances(sb1 + sb2) == sb[0] as int + total_balances(sb1[1..] + sb2);
+    //         distBalancesProp(sb1[1..],sb2);
+
+    //     }
+    // }
+
+    // lemma distDepositsProp(sd1: seq<Deposit>, sd2: seq<Deposit>)
+    //     ensures total_deposits(sd1 + sd2) == total_deposits(sd1) + total_deposits(sd2) 
+    // {
+    //     if |sd2| == 0 {
+    //         assert sd1 + sd2 == sd1;
+    //     }
+    //     else {
+    //         var sd := sd1 + sd2;
+    //         //assert sd == sd1 + sd2[..|sd2|-1] +  [sd2[|sd2|-1]];
+    //         assert sd[..|sd|-1] == sd1 + sd2[..|sd2|-1] ;
+    //         assert total_deposits(sd) == total_deposits(sd[..|sd|-1]) + sd2[|sd2|-1].data.amount as int;
+    //         //assert total_deposits(sd1 + sd2) == total_deposits(sd1 + sd2[..|sd2|-1] ) + sd2[|sd2|-1].data.amount as int;
+    //         distDepositsProp(sd1, sd2[..|sd2|-1] );
+    //     }
+    // }
+    // lemma subsetDepositSumProp(deposits: seq<Deposit>, i: nat)
+    //     requires i <= |deposits|
+    //     ensures total_deposits(deposits[..i]) <= total_deposits(deposits);
+    // {
+    //     if i == |deposits| {
+    //         assert deposits[..i] == deposits;
+    //     }
+    //     else {
+    //         //assert i < |deposits|;
+    //         assert deposits == deposits[..i] + deposits[i..];
+    //         assert total_deposits(deposits) == total_deposits(deposits[..i] + deposits[i..]);
+    //         distDepositsProp(deposits[..i], deposits[i..]);
+    //         //assert total_deposits(deposits[..i] + deposits[i..]) == total_deposits(deposits[..i]) + total_deposits(deposits[i..]); 
+    //     }
+    // }
+
+    
+
+}
