src/dafny/beacon/statetransition/ProcessOperations.dfy
@@ -24,6 +24,7 @@ include "../attestations/AttestationsTypes.dfy"
 include "../Helpers.dfy"
 include "StateTransition.s.dfy"
 include "../attestations/AttestationsHelpers.dfy"
+include "ProcessOperations.s.dfy"
 
 /**
  * State transition function for the Beacon Chain.
@@ -43,6 +44,8 @@ module ProcessOperations {
     import opened BeaconHelpers
     import opened StateTransitionSpec
     import opened AttestationsHelpers
+    import opened ProcessOperationsSpec
+    
 
     /**
      *  Process the operations defined by a block body.
@@ -51,7 +54,7 @@ module ProcessOperations {
      *  @param  bb  A block body.
      *  @returns    The state obtained after applying the operations of `bb` to `s`.
      */
-        method process_operations(s: BeaconState, bb: BeaconBlockBody)  returns (s' : BeaconState) 
+    method process_operations(s: BeaconState, bb: BeaconBlockBody)  returns (s' : BeaconState) 
         requires s.eth1_deposit_index as int +  |bb.deposits| < 0x10000000000000000 
         requires |s.validators| + |bb.deposits| <= VALIDATOR_REGISTRY_LIMIT as int
         requires |s.validators| == |s.balances|
